

# LaplaceTransformsExam3

Joel Boynton

November 17, 2025

## Part 1: Practice Problems

### Question 1 (Inverse Laplace - Partial Fractions)

The inverse Laplace transform of the function

$$F(s) = \frac{5s + 4}{(s - 1)(s + 2)}$$

is the function  $f(t)$ . Find the value of  $f(0)$ .

### Question 2 (Inverse Laplace - Quadratic Denominators)

The inverse Laplace transform of the function

$$F(s) = \frac{3s^2}{(s^2 + 1)(s^2 + 4)}$$

is the function  $f(t)$ . Find the value of  $f(\pi/2)$ .

### Question 3 (IVP - Non-Homogeneous)

Let  $y(t)$  be the solution to the initial value problem:

$$y'' - 3y' + 2y = 6e^{3t}$$

with initial conditions  $y(0) = 1$  and  $y'(0) = 3$ . Find the value of  $y(\ln 2)$ .

### Question 4 (IVP - Coefficient Sum)

Let  $y(t)$  be the solution to the initial value problem:

$$y'' - 4y' + 3y = e^{2t}$$

with initial conditions  $y(0) = 2$  and  $y'(0) = 3$ . The solution can be written in the form  $y(t) = Ae^t + Be^{3t} + Ce^{2t}$ . Find the value of the sum of the coefficients:  $A + B + C$ .

### Question 5 (Shifted Laplace)

Let  $f(t)$  be the inverse Laplace transform of:

$$F(s) = \frac{5e^{-2s}}{(s-4)^2}$$

Find the value of  $\frac{f(3)}{e^4}$ .

## Part 2: Solutions & Answer Key

### Solution to Question 1

We must find the partial fraction decomposition to determine  $f(t)$ , then evaluate at  $t = 0$ .

$$\frac{5s+4}{(s-1)(s+2)} = \frac{A}{s-1} + \frac{B}{s+2}$$

Find  $A$  (cover-up method at  $s = 1$ ):

$$A = \frac{5(1)+4}{1+2} = \frac{9}{3} = 3$$

Find  $B$  (cover-up method at  $s = -2$ ):

$$B = \frac{5(-2)+4}{-2-1} = \frac{-6}{-3} = 2$$

So,  $f(t) = 3e^t + 2e^{-2t}$ . Evaluate at  $t = 0$ :

$$f(0) = 3e^0 + 2e^0 = 3 + 2 = 5$$

**Answer: 5**

### Solution to Question 2

We assume the form:

$$\frac{3s^2}{(s^2+1)(s^2+4)} = \frac{A}{s^2+1} + \frac{B}{s^2+4}$$

Multiply by common denominator and substitute  $x = s^2$ :

$$3x = A(x+1) + B(x+1)$$

At  $x = -1$ :  $-3 = A(3) \implies A = -1$ . At  $x = -4$ :  $-12 = B(-3) \implies B = 4$ .

$$F(s) = \frac{-1}{s^2+1} + \frac{4}{s^2+4}$$

Inverse Laplace (remember  $\mathcal{L}^{-1}[\frac{\omega}{s^2+\omega^2}] = \sin(\omega t)$ ):

$$f(t) = -\sin(t) + \frac{4}{2} \sin(2t) = -\sin(t) + 2\sin(2t)$$

Evaluate at  $t = \pi/2$ :

$$\begin{aligned} f(\pi/2) &= -\sin(\pi/2) + 2\sin(\pi) \\ f(\pi/2) &= -1 + 2(0) = -1 \end{aligned}$$

**Answer: -1**

### Solution to Question 3

1. **Homogeneous:**  $r^2 - 3r + 2 = (r - 1)(r - 2) = 0 \implies y_h = c_1 e^t + c_2 e^{2t}$ .

2. **Particular:** Guess  $y_p = C e^{3t}$ .

$$(9C - 3(3C) + 2C)e^{3t} = 6e^{3t} \implies 2C = 6 \implies C = 3$$

General Solution:  $y = c_1 e^t + c_2 e^{2t} + 3e^{3t}$ . Derivative:  $y' = c_1 e^t + 2c_2 e^{2t} + 9e^{3t}$ .

3. **Initial Conditions:**  $y(0) = c_1 + c_2 + 3 = 1 \implies c_1 + c_2 = -2$   $y'(0) = c_1 + 2c_2 + 9 = 3 \implies c_1 + 2c_2 = -6$  Subtract equations:  $c_2 = -4$ . Solve for  $c_1$ :  $c_1 - 4 = -2 \implies c_1 = 2$ . Full Solution:  $y(t) = 2e^t - 4e^{2t} + 3e^{3t}$ .

4. **Evaluate:**  $y(\ln 2) = 2e^{\ln 2} - 4e^{2\ln 2} + 3e^{3\ln 2}$  Using  $e^{k \ln x} = x^k$ :  $y(\ln 2) = 2(2) - 4(4) + 3(8)$   
 $y(\ln 2) = 4 - 16 + 24 = 12$ .

**Answer: 12**

### Solution to Question 4

1. **Homogeneous:**  $r^2 - 4r + 3 = (r - 1)(r - 3) \implies y_h = A e^t + B e^{3t}$ .

2. **Particular:** Guess  $y_p = C e^{2t}$ .

$$(4C - 8C + 3C)e^{2t} = e^{2t} \implies -C = 1 \implies C = -1$$

$$y = A e^t + B e^{3t} - e^{2t}. \quad y' = A e^t + 3B e^{3t} - 2e^{2t}.$$

3. **Initial Conditions:**  $y(0) = A + B - 1 = 2 \implies A + B = 3$ .  $y'(0) = A + 3B - 2 = 3 \implies A + 3B = 5$ . Subtract:  $2B = 2 \implies B = 1$ . Solve for  $A$ :  $A + 1 = 3 \implies A = 2$ . Coefficients are  $A = 2, B = 1, C = -1$ .

4. **Sum:**  $A + B + C = 2 + 1 + (-1) = 2$ .

**Answer: 2**

### Solution to Question 5

Base function inverse:  $\mathcal{L}^{-1} \left\{ \frac{5}{(s-4)^2} \right\} = 5te^{4t}$ . Apply time shift  $t \rightarrow (t - 2)$  due to  $e^{-2s}$ :  $f(t) = 5(t - 2)e^{4(t-2)}u(t - 2)$ . Evaluate at  $t = 3$  (note:  $u(3 - 2) = u(1) = 1$ ):  $f(3) = 5(3 - 2)e^{4(3-2)} = 5(1)e^4 = 5e^4$ . Compute ratio:  $\frac{5e^4}{e^4} = 5$ . **Answer: 5**